### Introduction to Enumerative Combinatorics, quiz 2

#### Question 1

Let 

$$A = (1+1)^{10} = 2^{10} = \sum_{k=0}^{10} \binom{10}{k} (1)^{10-k} (1)^{k}$$

$$B = (-1 + 1)^{10} = 0 = \sum_{k=0}^{10} \binom{10}{k} (-1)^{10-k} (1)^{k}$$

$$$
A + B = 2^{10} = 2 * (\binom{10}{0} + \binom{10}{2} + \binom{10}{4} + ... + \binom{10}{10})
$$$

Therefore,

$$$
\binom{10}{0} + \binom{10}{2} + \binom{10}{4} + ... + \binom{10}{10} = 2^{9} = 512
$$$


#### Question 2

$$$
(a+b)^{n} = \sum_{k=0}^{n}\binom{n}{k}a^{n-k}b^{k}
$$$

$$$a = 1, b = 2$$$
$$$
3^{n} = \sum_{k=0}^{n}\binom{n}{k}2^{k}
$$$

#### Question 3
$$$
\frac{6!}{2!}
$$$

#### Question 4
$$$
\frac{7!}{3!}
$$$

#### Question 5

$$$
\frac{\frac{7!}{7}}{2}
$$$
